已知命题， (R≥ 0) ，使 (4x²+(a-2)x+(1)/(4)=0) 是假命题，则命题成立的必要不充分条件为

A. ((a≤ 0)) 或 (R∈ R) (4x²+(a-2)x+(1)/(4)=0) 是假命题，则命题成立的必要不充分条件为

B. ((a≥ 4)) 或 (4x²+(a-2)x+(1)/(4)≥ 0) 或 (4x²+(a-2)x+(1)/(4)≤ 0) 或 (4x²+(a-2)x+(1)/(4)>0) 或 (4x²+(a-2)x+(1)/(4)<0)

C. ((a≥ 4)) 或 (4x²+(a-2)x+(1)/(4)≥ 0) 或 (4x²+(a-2)x+(1)/(4)≤ 0) 或 (4x²+(a-2)x+(1)/(4)>0) 或 (4x²+(a-2)x+(1)/(4)<0) 或 (4x²+(a-2)x+(1)/(4)=0) 或 (4x²+(a-2)x+(1)/(4)≠ 0) 或 (4x²+(a-2)x+(1)/(4)≠ 0) 或 (a²-4a+4<0) 或 (a²-4a+4>0) 或 (a²-4a+4≥ 0) 或 (a²-4a+4≤ 0) 或 (a²-4a+4≠ 0) 或 (a²-4a+4=0) 或 (a²-4a+4<0) 或 (a²-4a+4>0) 或 (a²-4a+4≥ 0) 或 (a²-4a+4≤ 0) 或 (a²-4a+4≠ 0) 或 (a